theories/AStack.v
@@ -1,0 +1,70 @@
+Require Import Nat List IR.
+Import ListNotations.
+
+(** Model of lazy_wspace::ir::AbstractStack.
+
+    To simplify the proofs, it assumes an infinite stack capacity and does not
+    use checked addition like Rust. *)
+
+Variant lazy_size : Type :=
+  | Finite (n : nat)
+  | EmptyLit.
+
+Variant result (A : Type) : Type :=
+  | Ok (a : A)
+  | EmptyLitError.
+Arguments Ok {_}.
+Arguments EmptyLitError {_}.
+
+Record astack : Type := AStack {
+  values : list node;
+  guards : list (nat * node);
+  accessed : nat;
+  dropped : nat;
+  lazy_dropped : lazy_size;
+}.
+
+Definition make : astack :=
+  AStack [] [] 0 0 (Finite 0).
+
+Definition set_values (s : astack) (v : list node) : astack :=
+  let (_, g, a, d, l) := s in AStack v g a d l.
+Definition set_guards (s : astack) (g : list (nat * node)) : astack :=
+  let (v, _, a, d, l) := s in AStack v g a d l.
+Definition set_accessed (s : astack) (a : nat) : astack :=
+  let (v, g, _, d, l) := s in AStack v g a d l.
+Definition set_dropped (s : astack) (d : nat) : astack :=
+  let (v, g, a, _, l) := s in AStack v g a d l.
+Definition set_lazy_dropped (s : astack) (l : lazy_size) : astack :=
+  let (v, g, a, d, _) := s in AStack v g a d l.
+
+Definition push (s : astack) (v : node) : astack :=
+  set_values s (v :: s.(values)).
+
+Fixpoint get_guard' (guards : list (nat * node)) (n : nat) : option node :=
+  match guards with
+  | (gn, g) :: guards' =>
+      if n <=? gn then Some g
+      else get_guard' guards' n
+  | [] => None
+  end.
+Definition get_guard (s : astack) (n : nat) : option node :=
+  get_guard' s.(guards) n.
+
+Definition TODO := Ok (Err 42).
+
+Definition at_lazy (s : astack) (n : nat) : (astack * result node) :=
+  match nth_error s.(values) n with
+  | Some v => (s, Ok v)
+  | None =>
+      let n := n - length s.(values) in
+      match s.(lazy_dropped) with
+      | Finite l =>
+          let i := s.(dropped) + l + n in
+          match get_guard s (i + 1) with
+          | Some g => (s, TODO) (* StackRef i g *)
+          | None => (s, TODO) (* CheckedStackRef i *)
+          end
+      | EmptyLit => (s, EmptyLitError)
+      end
+  end.
